\title{\vspace{-2.0cm} 60006 - Tutorial 3

Interest Point Detection}
\author{
        Xin Wang
}
\date{\today}

\documentclass[12pt]{article}
\usepackage[margin=0.5in]{geometry} 
\usepackage{amsmath} 
\usepackage{graphicx}  
\usepackage[parfill]{parskip}

\setlength{\parindent}{0em}

\begin{document}
\maketitle

\section*{Question 1}

\textbf{Question 1.1:} Please derive the eigenvalues for this matrix.

\begin{gather*}
    \text{det} \left( \begin{pmatrix}
        3 & 1 \\ 1 & 3
    \end{pmatrix} - \lambda \begin{pmatrix}
        1 & 0 \\ 0 & 1
    \end{pmatrix}\right): \lambda^2 - 6\lambda + 8 \\ 
    \lambda = 4 \quad \lambda = 2
\end{gather*}

\textbf{Question 1.2:} Please compute the Harris detector response.
\begin{align*}
    R &=\lambda_1 \lambda_2 - k(\lambda_1 + \lambda_2)^2 \\
    &= 4*2 - 0.05(4 + 2)^2 \\ 
    &= 6.2
\end{align*}

\textbf{Question 1.3:} Please derive the eigenvalues for this matrix and the corresponding Harris
detector response. 
\begin{gather*}
    M = \begin{bmatrix}
        12 & 4 \\ 4 & 12
    \end{bmatrix} \\ 
    \lambda_1 = 16 \quad \lambda_2 = 8 \\ 
    R = 16*8 - 0.05(16 + 8)^2 = 99.2
\end{gather*}

\textbf{Question 1.4:} Directly calculate the scale-adapted Harris detector using trace and determinant instead of eigen decomposition. 
\begin{gather*}
    \text{det}(M) = 128 \\ 
    \text{tr}(M) = 24 \\ 
    R = \text{det}(M) - k(\text{tr}(M))^2 = 128 - 0.05(24)^2 = 99.2
\end{gather*}

\section*{Question 2}

\textbf{Question 2.1:} Please prove the following equation holds (also known as the heat diffusion equation). 
\begin{gather*}
    G(x,y,\sigma) = \frac{1}{2 \pi \sigma^2} e^{-\frac{x^2 + y^2}{2\sigma^2}} \\ 
\end{gather*}
\begin{align*}
    \frac{\partial G}{\partial \sigma} &= \dfrac{\left(y^2+x^2\right)\mathrm{e}^{-\frac{y^2+x^2}{2{\sigma}^2}}}{2{\pi}{\sigma}^5}-\dfrac{\mathrm{e}^{-\frac{y^2+x^2}{2{\sigma}^2}}}{{\pi}{\sigma}^3} \\
    &= -\dfrac{\left(2{\sigma}^2-y^2-x^2\right)}{2{\pi}{\sigma}^5}\mathrm{e}^{-\frac{y^2+x^2}{2{\sigma}^2}}
\end{align*}
\begin{gather*}
    \frac{\partial^2 G}{\partial x^2} = \dfrac{\left(x^2-{\sigma}^2\right)\mathrm{e}^{-\frac{x^2+y^2}{2{\sigma}^2}}}{2{\pi}{\sigma}^6} \\ 
    \frac{\partial^2 G}{\partial y^2} = \dfrac{\left(y^2-{\sigma}^2\right)\mathrm{e}^{-\frac{y^2+x^2}{2{\sigma}^2}}}{2{\pi}{\sigma}^6}
\end{gather*}

\textbf{Question 2.2}: 
\begin{gather*}
    \frac{\partial G}{\partial\sigma} \approx \sigma \nabla^2 G \quad \text{ and } \quad \frac{\partial G}{\partial\sigma} \approx \frac{G(k\sigma - G(\sigma))}{k\sigma - \sigma}\\ 
    DoG(x,y,\sigma) = G(k\sigma) - G(\sigma) \approx (k-1)\sigma^2 \nabla^2 G
\end{gather*}

\end{document}
